first spec for gen mem

ifc/extended/Testing/Generation.v
@@ -551,23 +551,26 @@ Definition gen_top : Gen Label :=
 
 (* Generates a memory adhering to the above constants *)
 (* Stamps are bottom everywhere - to be created later *)
-Definition gen_init_mem (top : Label) : Gen (memory * list (mframe * Z)) :=
-  bindGen (choose (C.min_no_frames, 
-                      C.max_no_frames)) (fun no_frames => 
-  let fix aux (n : nat) (ml : memory * list (mframe * Z)) := 
-      match n with
-        | O    => returnGen ml
-        | S n' => 
-          let (m, l) := ml in
-          bindGen (choose (C.min_frame_size,
-                            C.max_frame_size)) (fun frame_size =>
-          bindGen (gen_label top) (fun lab =>
-          match (alloc frame_size lab bot (Vint Z0 @ bot) m) with
-            | Some (mf, m') => aux n' (m', (mf,frame_size) :: l)
-            | None => aux n' ml
-          end))
-      end in
-  aux no_frames (Mem.empty Atom Label, [])).
+
+Fixpoint gen_init_mem_helper top (n : nat) (m : memory) :=
+  match n with
+    | O    => returnGen m
+    | S n' =>
+      bindGen (choose (C.min_frame_size,
+                       C.max_frame_size)) (fun frame_size =>
+      bindGen (gen_label top) (fun lab =>
+        match (alloc frame_size lab bot (Vint Z0 @ bot) m) with
+          | Some (_, m') =>
+            gen_init_mem_helper top n' m'
+          | None => gen_init_mem_helper top n' m
+        end))
+  end.
+
+
+Definition gen_init_mem (top : Label) : Gen memory :=
+  bindGen (choose (C.min_no_frames,
+                      C.max_no_frames)) (fun no_frames =>
+  gen_init_mem_helper top no_frames (Mem.empty Atom Label)).
 
 Definition failed_state : State :=
   Property.trace "Failed State!" 
@@ -591,14 +594,25 @@ Definition populate_memory inf (m : memory) : Gen memory :=
 (* FIX this to instantiate stamps to a non-trivially well-formed state *)
 Definition instantiate_stamps (st : State) : State := st.
 
+Definition get_blocks_and_sizes (top : Label) (m : memory) :=
+  map 
+    (fun b => 
+    let length := 
+        match Mem.get_frame m b with
+          | Some fr => 
+            let 'Fr _ _ data := fr in length data 
+          | _ => 0 
+        end in (b, Z.of_nat length)) (Mem.get_all_blocks top m).
+
+
 (* Generate an initial state.
    TODO : Currently stamps are trivially well formed (all bottom) *)
 Definition gen_variation_state : Gen (@Variation State) :=
   (* Generate basic machine *)
   bindGen gen_top (fun prins =>            
   (* Generate initial memory and dfs *)
-  bindGen (gen_init_mem prins) (fun init_mem_info =>
-  let (init_mem, dfs) := init_mem_info in
+  bindGen (gen_init_mem prins) (fun init_mem =>
+  let dfs := get_blocks_and_sizes prins init_mem in
   (* Generate initial instruction list *)
   let imem := replicate (C.code_len) Nop in
   (* Create initial info - if this fails, fail the generation *)
